Lp2lc/Active/package.lean
@@ -3,3 +3,4 @@
 import «Lp2lc».Active.STLC.Def
 import «Lp2lc».Active.STLC.Proof
 import «Lp2lc».Active.STLC.SI.Proof
+import «Lp2lc».Active.STLC.SI.Proof_NoEnvInTerm
